verif/verif_dlinklist_proof1.v
@@ -1,0 +1,401 @@
+Require Import VST.floyd.proofauto.
+Require Import VST.floyd.Funspec_old_Notation.
+Require Import DL.verif.dlinklist.
+Require Import DL.verif.verif_dlinklist_def.
+
+Instance CompSpecs : compspecs. make_compspecs prog. Defined.
+Definition Vprog : varspecs. mk_varspecs prog. Defined.
+
+Local Open Scope logic.
+
+(***********************************************************************
+V.Main proofs
+***********************************************************************)
+
+(* 
+Lemma list_1n_rep_saturate_local_nullprev_tail:
+  forall l head tail, 
+    list_1n_rep l head tail nullval |-- 
+    !! is_pointer_or_null tail.
+Proof.
+  intros. 
+  pose proof (list_1n_rep_saturate_local_tail l head tail nullval
+    mapsto_memory_block.is_pointer_or_null_nullval).
+  exact H.
+Qed.
+Hint Resolve list_1n_rep_saturate_local_nullprev_tail: saturate_local.
+ *)
+Lemma list_head_null : forall l tail prev, 
+  list_1n_rep l nullval tail prev |-- !! (l = nil) && emp.
+Proof.
+  intros.
+  destruct l.
+  - simpl. entailer!.
+  - simpl. Intros old_head. unfold node_rep. 
+    entailer!. 
+    sfcn.
+Qed.
+
+Lemma Z_length_minus_1 : forall a l, Z_length (a :: l) - 1 = Z_length l.
+Proof.
+  intros.
+  unfold Z_length.
+  simpl length.
+  lia.
+Qed.
+
+Lemma Z_length_plus_1 : forall a l, (Z_length l) + 1 = Z_length (a :: l).
+Proof.
+  intros.
+  unfold Z_length.
+  simpl length.
+  lia.
+Qed.
+
+(* proof for next *)
+Theorem body_next: 
+  semax_body Vprog Gprog f_next next_spec.
+Proof.
+  start_function.
+  unfold node_rep.
+  forward.
+(* return p->next; *)
+(* proof for begin *)
+Abort.
+
+Theorem body_begin: 
+  semax_body Vprog Gprog f_begin begin_spec.
+Proof.
+  start_function. 
+  unfold list_rep.
+  Intros head tail.
+  forward.
+  forward.                              (* return l->head; *)
+  unfold list_single_out.
+  destruct (list_nth_out l 0) as [[l1 y] l2] eqn:E.
+  destruct y.
+  - (* not an empty linklist *)
+    destruct l.
+    { (* show that l <> [] *)
+      rewrite list_nth_nil in E.
+      inversion E.
+    }
+    simpl in E; inversion E; subst.
+    simpl list_1n_rep_aux.
+    simpl list_1n_rep.
+    Intros old_head.
+    Exists head head tail nullval nullval old_head tail.
+    entailer!.
+  - (* an empty linklist *)
+    destruct l; [| inversion E].
+    destruct H; subst.
+    simpl in E; inversion E; subst.
+    simpl list_1n_rep.
+    Intros; subst.
+    Exists nullval nullval nullval.
+    entailer!.
+    apply TT_right. 
+Qed.
+
+(* proof for end *)
+Theorem body_end: 
+  semax_body Vprog Gprog f_end end_spec.
+Proof.
+  start_function. 
+  unfold list_rep.
+  Intros head tail.
+  forward.
+  { (* TODO: is there some shadowing? *)
+    pose proof (list_1n_rep_saturate_local_tail l head tail nullval
+    mapsto_memory_block.is_pointer_or_null_nullval).
+    sep_apply H.
+    entailer!.
+  }
+  forward.                              (* return l->tail; *)
+  unfold list_single_out.
+  destruct (list_nth_out l ((length l) - 1)%nat) as [[l1 y] l2] eqn:E.
+  destruct y.
+  - (* not an empty linklist *)
+    destruct l.
+    { (* show that l <> [] *)
+      rewrite list_nth_nil in E.
+      inversion E.
+    }
+    pose proof (list_cons_app l z0).
+    destruct H1 as [l3 [a H1]].
+    destruct H1 as [H1 [H2 H3]].
+    rewrite H1.
+    sep_apply list_1n_split.
+    Intros head' tail'.
+    simpl list_1n_rep at 1.
+    Intros old_head.
+    Exists head' head tail.
+    Exists head tail' old_head tail.
+    pose proof E.
+    apply list_nth_tail in E. subst l2.
+    simpl_length.
+    apply list_nth_split in H6.
+    destruct H6 as [H6 H7].
+    rewrite <- H3 in H7.
+    rewrite <- H2 in H6.
+    simpl list_1n_rep.
+    inversion H7; subst.
+    entailer!.
+  - (* empty linklist *)
+    Exists nullval head tail.
+    destruct l.
+    2: {
+      simpl_length.
+      apply list_nth_split in E.
+      destruct E.
+      pose proof (list_cons_app l z).
+      repeat destruct H3.
+      rewrite <- (proj2 H4) in H2.
+      discriminate.
+    }
+    simpl in E; inversion E; subst.
+    simpl list_1n_rep.
+    Intros; subst.
+    entailer!.
+    apply TT_right. 
+Qed.
+
+(* proof for rend, the same as begin *)
+Theorem body_rend: 
+  semax_body Vprog Gprog f_rend rend_spec.
+Proof.
+  start_function. 
+  unfold list_rep.
+  Intros head tail.
+  forward.
+  forward.                              (* return l->head; *)
+  unfold list_single_out.
+  destruct (list_nth_out l 0) as [[l1 y] l2] eqn:E.
+  destruct y.
+  - (* not an empty linklist *)
+    destruct l.
+    { (* show that l <> [] *)
+      rewrite list_nth_nil in E.
+      inversion E.
+    }
+    simpl in E; inversion E; subst.
+    simpl list_1n_rep_aux.
+    simpl list_1n_rep.
+    Intros old_head.
+    Exists head head tail nullval nullval old_head tail.
+    entailer!.
+  - (* an empty linklist *)
+    destruct l; [| inversion E].
+    destruct H; subst.
+    simpl in E; inversion E; subst.
+    simpl list_1n_rep.
+    Intros; subst.
+    Exists nullval nullval nullval.
+    entailer!.
+    apply TT_right. 
+Qed.
+
+(* proof for rbegin, the same as end *)
+Theorem body_rbegin: 
+  semax_body Vprog Gprog f_rbegin rbegin_spec.
+Proof.
+  start_function. 
+  unfold list_rep.
+  Intros head tail.
+  forward.
+  { (* TODO: is there some shadowing? *)
+    pose proof (list_1n_rep_saturate_local_tail l head tail nullval
+    mapsto_memory_block.is_pointer_or_null_nullval).
+    sep_apply H.
+    entailer!.
+  }
+  forward.                              (* return l->tail; *)
+  unfold list_single_out.
+  destruct (list_nth_out l ((length l) - 1)%nat) as [[l1 y] l2] eqn:E.
+  destruct y.
+  - (* not an empty linklist *)
+    destruct l.
+    { (* show that l <> [] *)
+      rewrite list_nth_nil in E.
+      inversion E.
+    }
+    pose proof (list_cons_app l z0).
+    destruct H1 as [l3 [a H1]].
+    destruct H1 as [H1 [H2 H3]].
+    rewrite H1.
+    sep_apply list_1n_split.
+    Intros head' tail'.
+    simpl list_1n_rep at 1.
+    Intros old_head.
+    Exists head' head tail.
+    Exists head tail' old_head tail.
+    pose proof E.
+    apply list_nth_tail in E. subst l2.
+    simpl_length.
+    apply list_nth_split in H6.
+    destruct H6 as [H6 H7].
+    rewrite <- H3 in H7.
+    rewrite <- H2 in H6.
+    simpl list_1n_rep.
+    inversion H7; subst.
+    entailer!.
+  - (* empty linklist *)
+    Exists nullval head tail.
+    destruct l.
+    2: {
+      simpl_length.
+      apply list_nth_split in E.
+      destruct E.
+      pose proof (list_cons_app l z).
+      repeat destruct H3.
+      rewrite <- (proj2 H4) in H2.
+      discriminate.
+    }
+    simpl in E; inversion E; subst.
+    simpl list_1n_rep.
+    Intros; subst.
+    entailer!.
+    apply TT_right. 
+Qed.
+
+(* proof for get_size *)
+Theorem body_get_size: 
+  semax_body Vprog Gprog f_get_size get_size_spec.
+Proof.
+  start_function. 
+  unfold list_rep.
+  Intros head tail.
+  forward.
+  forward.
+  unfold list_rep.
+  Exists head tail.
+  entailer!.
+Qed.
+(* 
+Definition list_new_spec :=
+ DECLARE _list_new
+  WITH u : unit
+  PRE  [  ]
+       PROP() LOCAL() SEP ()
+  POST [ tptr t_struct_list ]
+    EX v: val,
+    PROP ()
+    LOCAL (temp ret_temp v)
+    SEP (list_rep nil v).
+ *)
+(* proof for list_new *)
+Theorem body_list_new: 
+  semax_body Vprog Gprog f_list_new list_new_spec.
+Proof.
+  start_function.
+  forward_call (sizeof t_struct_list).  (* mallocN *)
+  { computable. }
+  Intros p.
+  rewrite memory_block_data_at_ by auto.
+  forward.                              (* l->head = NULL;  *)
+  forward.                              (* l->tail = NULL;  *)
+  forward.                              (* l->size = 0;     *)
+  forward.                              (* return;          *)
+  Exists p. 
+  entailer.
+  unfold list_rep. 
+  Exists nullval nullval.
+  simpl list_1n_rep.
+  entailer!.
+Qed.
+
+(* proof for list_free *)
+Theorem body_list_free: 
+  semax_body Vprog Gprog f_list_free list_free_spec.
+Proof.
+  start_function.
+  unfold list_rep.
+  Intros head tail.
+  forward.                              (* tmp = l->head;   *)
+  forward_while
+  ( EX l' : list Z, EX head' : val, 
+    EX prev' : val, 
+    PROP ()
+    LOCAL (temp _l p; temp _tmp head')
+    SEP (data_at Tsh t_struct_list 
+      (Vint (Int.repr (Z_length l')), (head', tail)) p * 
+      list_1n_rep l' head' tail prev'))%assert.
+  { Exists l head nullval. entailer!. }
+  { destruct l'; entailer!. }
+  { (* loop body *)
+    destruct l'.
+    { simpl. Intros. contradiction. }
+    simpl. unfold node_rep. Intros old_head.
+    forward.
+    forward.                            (* l->head = tmp->next; *) 
+    forward_call (head', sizeof t_struct_node); [solve_free | ].
+                                        (* freeN(tmp, sizeof (struct node)); *)
+    forward.
+    forward.                            (* l->size -= 1;    *)
+    forward.                            (* tmp = l->head;   *)
+    Exists (l', old_head, head').
+    entailer!.
+    rewrite Z_length_minus_1.
+    entailer!.
+  }
+  subst head'.
+  sep_apply list_head_null.
+  Intros.
+  forward_call (p, sizeof t_struct_list); [solve_free | ].
+                                        (* freeN(l, sizeof (struct list)); *)
+  entailer!.
+Qed.
+
+
+(* 
+Definition begin_spec :=
+ DECLARE _begin
+  WITH p : val, l : list Z
+  PRE  [ _l OF (tptr t_struct_list) ]
+    PROP () 
+    LOCAL (temp _l p) 
+    SEP (list_rep l p)
+  POST [ tptr t_struct_node ]
+    EX res : val, EX head : val, EX tail : val, 
+    PROP ()
+    LOCAL (temp ret_temp res)
+    SEP (data_at Tsh t_struct_list
+          (Vint (Int.repr (Z_length l)), (head, tail)) p; 
+          list_single_out l 0%nat res).
+ *)
+Theorem body_begin_ref: 
+  semax_body Vprog Gprog f_begin begin_spec.
+Proof.
+  start_function. 
+  unfold list_rep.
+  Intros head tail.
+  forward.
+  forward.                              (* return l->head; *)
+  unfold list_single_out. 
+
+  
+  destruct (list_nth_out l 0) as [[l1 y] l2] eqn:E.
+  destruct y.
+  - (* not an empty linklist *)
+    destruct l.
+    { (* show that l <> [] *)
+      rewrite list_nth_nil in E.
+      inversion E.
+    }
+    simpl in E; inversion E; subst.
+    simpl list_1n_rep_aux.
+    simpl list_1n_rep.
+    Intros old_head.
+    Exists head head tail nullval nullval old_head tail.
+    entailer!.
+  - (* an empty linklist *)
+    destruct l; [| inversion E].
+    destruct H; subst.
+    simpl in E; inversion E; subst.
+    simpl list_1n_rep.
+    Intros; subst.
+    Exists nullval nullval nullval.
+    entailer!.
+    apply TT_right. 
+Qed.
+
