verif_ex/add_vrif.v
@@ -1,0 +1,10 @@
+Require Import VST.floyd.proofauto.
+(** This file is auxiliary tactics that we will use in this tutorial. *)
+Require Export VST.floyd.Funspec_old_Notation.
+
+(** These are the C programs that we will verify. *)
+Require EV.add EV.abs EV.append EV.max3 EV.swap EV.tri EV.gcd EV.fact EV.test_null EV.reverse.
+
+Local Open Scope logic.
+
+Module Verif_uadd.
