s
@@ -1,0 +1,97 @@
+[33mcommit 029eb80d8df7e2ca44d11b4248de3732a6cdcf2b[m[33m ([m[1;36mHEAD -> [m[1;32mbranch_zjl[m[33m, [m[1;32mmaster[m[33m)[m
+Author: TT885 <zhangjiale100@sjtu.edu.cn>
+Date:   Tue Jun 2 09:46:20 2020 +0800
+
+    zjl
+
+[33mcommit bd5aa9f007e64132326a379e3c8409eec3d2bef9[m[33m ([m[1;31morigin/master[m[33m, [m[1;31morigin/HEAD[m[33m)[m
+Author: zqy1018 <979115525@qq.com>
+Date:   Mon May 11 23:32:08 2020 +0800
+
+    removed list_full_rep
+
+[33mcommit e9489fe433f3f12abd203a3d4e6249612cf5ce2d[m
+Author: zqy1018 <979115525@qq.com>
+Date:   Mon May 11 22:57:36 2020 +0800
+
+    added some tips
+
+[33mcommit e514bd3d6455807872d303415c95ddd257b9299c[m
+Author: zqy1018 <979115525@qq.com>
+Date:   Mon May 11 22:52:41 2020 +0800
+
+    archived the topics and instructions
+
+[33mcommit 73b82c99923d0da63afef1c73e7ea5a7507fe86b[m
+Author: zqy1018 <979115525@qq.com>
+Date:   Mon May 11 22:50:22 2020 +0800
+
+    added .gitignore
+
+[33mcommit 9dc11a0e1fdd7551942d64ab8ab3f81b029cc0c0[m
+Author: zqy1018 <979115525@qq.com>
+Date:   Sat May 9 22:05:33 2020 +0800
+
+    fixed the rep of link list
+
+[33mcommit 31382dcab1711291cdb9c9c9aa70ecc4531ab349[m
+Author: zqy1018 <979115525@qq.com>
+Date:   Thu May 7 18:38:09 2020 +0800
+
+    Updated
+
+[33mcommit 077a1ba6bec3982e9eee14954ba7e370f784569c[m
+Author: zqy1018 <979115525@qq.com>
+Date:   Thu May 7 18:35:06 2020 +0800
+
+    write basic reps and solved malloc and free
+
+[33mcommit df91b2c010afb0077b0701c0c6d33e62fb5f6476[m
+Author: zqy1018 <979115525@qq.com>
+Date:   Sat May 2 23:55:16 2020 +0800
+
+    Added the C program
+
+[33mcommit 184b1060f3649cb1b0d7dcf474c84fc39ee402f4[m
+Author: zqy1018 <979115525@qq.com>
+Date:   Thu Apr 30 23:42:51 2020 +0800
+
+    Added the goal
+
+[33mcommit 86c26cac6b060b025cc015e44ceadb7f964e2c5d[m
+Author: zqy1018 <979115525@qq.com>
+Date:   Thu Apr 30 22:38:54 2020 +0800
+
+    Determined the topic
+
+[33mcommit 522d8911a8057aacac4ef0cbb0c69fa06d5b09e8[m
+Author: TT885 <48856945+TT885@users.noreply.github.com>
+Date:   Thu Apr 30 22:13:26 2020 +0800
+
+    Add files via upload
+
+[33mcommit 885d91a3e19a52fd5649090ec401a9959e168b8d[m
+Author: TT885 <48856945+TT885@users.noreply.github.com>
+Date:   Thu Apr 30 21:58:31 2020 +0800
+
+    Update README.md
+
+[33mcommit 042c8a69ef244cc2f78a13545347ed6d96b4ba54[m
+Author: TT885 <48856945+TT885@users.noreply.github.com>
+Date:   Thu Apr 30 21:56:23 2020 +0800
+
+    Update README.md
+
+[33mcommit 77cee472a2fb197034262a0d8d78128ed85da9fb[m
+Author: TT885 <48856945+TT885@users.noreply.github.com>
+Date:   Thu Apr 30 21:54:17 2020 +0800
+
+    Add files via upload
+    
+    大作业要求
+
+[33mcommit 7a8b577f0cd6672747cef67ee04baec83eccab09[m
+Author: sdlnwr <44577016+sdlnwr@users.noreply.github.com>
+Date:   Thu Apr 30 20:57:06 2020 +0800
+
+    Initial commit
